more refactoring

MultiScalarMul_Abstract.ec
@@ -60,6 +60,16 @@ axiom mul_plus_distr   : forall (a : int), forall (b c : R),
 
 
 
+lemma qiq : forall a, 0 <= a => forall (c : int), forall (b : R),
+   a *** b +++ c *** b = (a + c) *** b.
+apply natind. progress. smt.
+progress. rewrite nplus_dist. auto.
+have ->: (n + 1 + c) = ((n + c) + 1). smt().
+rewrite nplus_dist. 
+rewrite - H0. smt().    
+smt(op_comm op_assoc).
+qed.    
+
 lemma const_add_inj : forall (x y a : R), x +++ a = y +++ a <=> x = y.
 proof. progress.
 have q : (x +++ a) +++ - a = (y +++ a) +++ - a.
@@ -133,6 +143,97 @@ module type OutCalls = {
 }.
 
 
+op predicate (x : R) (r : R) = xof x <> xof r.
+(* check the U candidate  *)
+op u_check (r : R) : bool.
+
+(* check whether the table could be computed *)
+op table_check (P : int -> R) (r : R) : bool.
+
+
+op helperI_pure (l : int) (argT : int -> int -> R)
+  (args : int -> int -> int) (argic : int) (argcc : R) 
+    = (iteri l (fun j (acc : bool * R) 
+        => (acc.`1 /\ predicate acc.`2 (argT j (args j argic)) , acc.`2 %%% argT j (args j argic))) (true, argcc)).
+
+  
+op multiScalarMulII_pure (T l : int) (argT : int -> int -> R)
+  (args : int -> int -> int) (argu : R) (argw : int)
+    = (iteri T (fun i (acc : bool * R) 
+        => let r = helperI_pure l argT args i ((2 ^ argw) *** acc.`2) in (acc.`1 /\ r.`1, r.`2)) (true, argu)).
+
+
+
+module SimpleComp = {
+  proc doubleLoop(p : R, w : int) = {
+      var cnt;
+      cnt <- 0;
+      while (cnt < w) {
+        p <- p +++ p;
+        cnt <- cnt + 1;
+      }
+      return p;
+  }
+
+
+  proc incompleteAddLoop(acc : R, table : int -> int-> R, ic : int, s : int -> int -> int) =    {
+      var jc, aux, vahe, flag;
+    
+      aux <- witness;
+      flag <- true;
+      jc <- 0;
+      vahe <- acc;
+      while (jc < l) {
+        aux <- table jc (s jc ic);
+        flag <- flag /\ predicate vahe aux;
+        vahe <- (vahe %%% aux);
+
+        jc <- jc + 1;
+      }
+      return (flag, vahe);
+  }
+
+
+  proc multiScalarMulMain(P : int -> R, s : int -> int -> int, U : R, table : int -> int -> R ) = {
+    var acc, aux, result : R;
+
+    var ic, jc, cnt : int;
+    var flag, flagaux : bool;
+    flag    <- true;
+    flagaux <- true;
+    acc     <- l *** U;
+    ic      <- 0;
+    while (ic < T) {
+      acc <@ doubleLoop(acc,w);
+      (flagaux, acc) <@ incompleteAddLoop(acc, table, ic, s);
+      flag <- flag && flagaux;
+      ic <- ic + 1;
+    }    
+    return (flag, acc);
+  }
+
+  proc multiScalarMul_Fun(P : int -> R, s : int -> int -> int) = {
+    var u_cand, flag, result, table;
+
+    u_cand <$ r_distr;
+
+   (* check u *)
+   flag   <- u_check u_cand;
+
+   (* check table  *)
+   flag   <- flag /\ table_check P (u_cand);
+   table  <- perfect_table_pure  P ((2 ^ w - 1) *** ( u_cand));
+
+   (* do the double-and-add computation  *)
+   result <- multiScalarMulII_pure T l table s (l *** ( u_cand)) w;
+
+   return (flag /\ result.`1, result.`2 +++ (- (l *** ( u_cand))));
+  }
+
+
+}.
+
+
 module MultiScalarMul(O : OutCalls) = {
 
   proc helper(acc : int, table : int -> int-> int, ic : int, P : int -> int, s : int -> int -> int, U : int) = {
@@ -166,15 +267,15 @@ module MultiScalarMul(O : OutCalls) = {
 
 
 
-  proc doubleWtimes(p : R, w : int) = {
-      var cnt;
-      cnt <- 0;
-      while (cnt < w) {
-        p <- p +++ p;
-        cnt <- cnt + 1;
-      }
-      return p;
-  }
+  (* proc doubleWtimes(p : R, w : int) = { *)
+  (*     var cnt; *)
+  (*     cnt <- 0; *)
+  (*     while (cnt < w) { *)
+  (*       p <- p +++ p; *)
+  (*       cnt <- cnt + 1; *)
+  (*     } *)
+  (*     return p; *)
+  (* } *)
 
 
   
@@ -191,7 +292,7 @@ module MultiScalarMul(O : OutCalls) = {
 
     ic <- 0;
     while (ic < T) {
-      acc <@ doubleWtimes(acc,w);
+      acc <@ SimpleComp.doubleLoop(acc,w);
       acc <@ helperR(acc, table, ic, s);
       ic <- ic + 1;
     }
@@ -237,7 +338,7 @@ module MultiScalarMul(O : OutCalls) = {
 
     ic <- 0;
     while (ic < T) {
-      acc <@ doubleWtimes(acc,w);
+      acc <@ SimpleComp.doubleLoop(acc,w);
       (flagaux, acc) <@ helperI(acc, table, ic, s);
       flag <- flag && flagaux;
       ic <- ic + 1;
@@ -289,7 +390,7 @@ module MultiScalarMul(O : OutCalls) = {
     acc     <- l *** U;
     ic      <- 0;
     while (ic < T) {
-      acc <@ doubleWtimes(acc,w);
+      acc <@ SimpleComp.doubleLoop(acc,w);
       (flagaux, acc) <@ helperI(acc, table, ic, s);
       flag <- flag && flagaux;
       ic <- ic + 1;
@@ -312,17 +413,30 @@ op multiScalarMulR  (s : int -> int -> int) (P : int -> R)
 
 
 
-lemma qiq : forall a, 0 <= a => forall (c : int), forall (b : R),
-   a *** b +++ c *** b = (a + c) *** b.
-apply natind. progress. smt.
-progress. rewrite nplus_dist. auto.
-have ->: (n + 1 + c) = ((n + c) + 1). smt().
-rewrite nplus_dist. 
-rewrite - H0. smt().    
-smt(op_comm op_assoc).
-qed.    
 
 
 
+lemma doublewtimes_spec_ph argP argw :
+ phoare [ SimpleComp.doubleLoop : arg = (argP, argw) /\
+   0 <= argw  ==>  res = (2 ^ argw) *** argP  ] = 1%r.
+proc. 
+   while (cnt <= w /\ 0 <= argw /\ 0 <= cnt /\ p = (2 ^ cnt) *** argP) (w - cnt).
+move => z.    
+   wp.
+   skip. progress. smt(). smt().
+   rewrite qiq. smt.
+   have ->: (2 ^ cnt{hr} + 2 ^ cnt{hr}) = (2 * 2 ^ cnt{hr} ).
+   smt(@Int).
+   congr.
+   rewrite exprS. auto. auto.
+   smt().
+   wp. skip. progress. smt. smt().
+   smt(@Int).
+qed.
 
 
+lemma doublewtimes_spec argP argw :
+ hoare [ SimpleComp.doubleLoop : arg = (argP, argw) /\
+   0 <= argw  ==>  res = (2 ^ argw) *** argP  ].
+conseq (doublewtimes_spec_ph argP argw).   
+qed.   
